cryptis/primitives/pre_term.v
@@ -4,12 +4,17 @@
 
    Every pure function of [normalize.v] has a counterpart here:
 
-     is_inv / is_exp / is_mul / is_nonce   ->  hl_is_inv / hl_is_exp /
-                                               hl_is_mul / hl_is_nonce
-     base / expo / factors                 ->  hl_base / hl_expo / hl_factors
-     inv_aux / mul_aux                     ->  hl_inv_aux / hl_mul_aux
+     is_inv / is_ginv / is_exp             ->  hl_is_inv / hl_is_ginv /
+     is_mul / is_gmul / is_nonce               hl_is_exp / hl_is_mul /
+                                               hl_is_gmul / hl_is_nonce
+     base / expo                           ->  hl_base / hl_expo
+     factors / gfactors                    ->  hl_factors / hl_gfactors
+     inv_aux / ginv_aux                    ->  hl_inv_aux / hl_ginv_aux
+     mul_aux / gmul_aux                    ->  hl_mul_aux / hl_gmul_aux
      normalize_factors                     ->  hl_normalize_factors
+     normalize_gfactors                    ->  hl_normalize_gfactors
      mul / inv                             ->  hl_mul_list / hl_inv
+     gmul / ginv                           ->  hl_gmul_list / hl_ginv
      mk_exp / exp_aux / exp                ->  hl_mk_exp / hl_exp_aux / hl_exp
 
    [normalize] itself is not implemented: the HeapLang layer only ever builds
@@ -134,8 +139,14 @@ Definition hl_is_inv : val := λ: "pt",
 Definition hl_is_exp : val := λ: "pt",
   if: Fst "pt" = #TOp2_tag then Fst (Fst (Snd "pt")) = #TExp_tag else #false.
 
+Definition hl_is_ginv : val := λ: "pt",
+  if: Fst "pt" = #TOp1_tag then Fst (Fst (Snd "pt")) = #TGInv_tag else #false.
+
 Definition hl_is_mul : val := λ: "pt",
   if: Fst "pt" = #TOpN_tag then Fst (Snd "pt") = #TMul_tag else #false.
+
+Definition hl_is_gmul : val := λ: "pt",
+  if: Fst "pt" = #TOpN_tag then Fst (Snd "pt") = #TGMul_tag else #false.
 
 Definition hl_is_nonce : val := λ: "pt",
   if: Fst "pt" = #TOp0_tag then Fst (Snd "pt") = #TNonce_tag else #false.
@@ -151,14 +162,23 @@ Definition hl_base : val := λ: "pt",
 Definition hl_expo : val := λ: "pt",
   if: hl_is_exp "pt" then Snd (Snd "pt") else hl_one.
 
+Definition hl_gone : val := (#TOpN_tag, (#TGMul_tag, NILV))%V.
+
 Definition hl_factors : val := λ: "pt",
   if: hl_is_mul "pt" then Snd (Snd "pt") else "pt" :: NILV.
+
+Definition hl_gfactors : val := λ: "pt",
+  if: hl_is_gmul "pt" then Snd (Snd "pt") else "pt" :: NILV.
 
 (** ** Smart constructors *)
 
 Definition hl_inv_aux : val := λ: "pt",
   if: hl_is_inv "pt" then Snd (Snd "pt")
   else (#TOp1_tag, (#TInv_tag, #(), "pt")).
+
+Definition hl_ginv_aux : val := λ: "pt",
+  if: hl_is_ginv "pt" then Snd (Snd "pt")
+  else (#TOp1_tag, (#TGInv_tag, #(), "pt")).
 
 Definition hl_mul_aux : val := λ: "c",
   match: "c" with
@@ -170,41 +190,66 @@ Definition hl_mul_aux : val := λ: "c",
       end
   end.
 
+Definition hl_gmul_aux : val := λ: "c",
+  match: "c" with
+    NONE => hl_gone
+  | SOME "x" =>
+      match: Snd "x" with
+        NONE => Fst "x"
+      | SOME <> => (#TOpN_tag, (#TGMul_tag, "c"))
+      end
+  end.
+
 (* [mbind PreTerm.factors]: flatten the factor lists of a list of pre-terms. *)
 Definition hl_all_factors : val := λ: "ts",
   foldr_list (λ: "t" "acc", append_lists (hl_factors "t") "acc") [] "ts".
+
+Definition hl_all_gfactors : val := λ: "ts",
+  foldr_list (λ: "t" "acc", append_lists (hl_gfactors "t") "acc") [] "ts".
 
 (* [PreTerm.normalize_factors] = [SMS.to pt_order inv_aux] of the flattened
    factors, so this is [sms_to] at the pre-term instance. *)
 Definition hl_normalize_factors : val := λ: "ts",
   sms_to leq_term eq_term hl_inv_aux (hl_all_factors "ts").
 
+Definition hl_normalize_gfactors : val := λ: "ts",
+  sms_to leq_term eq_term hl_ginv_aux (hl_all_gfactors "ts").
+
 Definition hl_mul_list : val := λ: "ts",
   hl_mul_aux (hl_normalize_factors "ts").
 
+Definition hl_gmul_list : val := λ: "ts",
+  hl_gmul_aux (hl_normalize_gfactors "ts").
+
 Definition hl_mul : val := λ: "t1" "t2", hl_mul_list ("t1" :: "t2" :: NILV).
+
+Definition hl_gmul : val := λ: "t1" "t2", hl_gmul_list ("t1" :: "t2" :: NILV).
 
 Definition hl_inv : val := λ: "t",
   if: hl_is_mul "t" then hl_mul_list (map_list hl_inv_aux (hl_factors "t"))
   else hl_inv_aux "t".
 
+Definition hl_ginv : val := λ: "t",
+  if: hl_is_gmul "t" then hl_gmul_list (map_list hl_ginv_aux (hl_gfactors "t"))
+  else hl_ginv_aux "t".
+
 Definition hl_mk_exp : val := λ: "b" "e",
   if: eq_term "e" hl_one then "b" else (#TOp2_tag, (#TExp_tag, "b", "e")).
 
-(* [exp_aux]: on a [PTInv] the inverse is stripped with [hl_inv_aux], the
-   exponent merged, and the inverse put back -- mirroring the [PTInv] branch of
-   [PreTerm.exp_aux]. *)
+(* [exp_aux]: on a [PTGInv] the group inverse is stripped with [hl_ginv_aux],
+   the exponent merged with the *scalar* [hl_mul_list], and the group inverse
+   put back -- mirroring the [PTGInv] branch of [PreTerm.exp_aux]. *)
 Definition hl_exp_aux : val := λ: "b" "e",
-  if: hl_is_inv "b" then
-    let: "u" := hl_inv_aux "b" in
-    hl_inv_aux (hl_mk_exp (hl_base "u")
+  if: hl_is_ginv "b" then
+    let: "u" := hl_ginv_aux "b" in
+    hl_ginv_aux (hl_mk_exp (hl_base "u")
                   (hl_mul_list (hl_expo "u" :: "e" :: NILV)))
   else hl_mk_exp (hl_base "b") (hl_mul_list (hl_expo "b" :: "e" :: NILV)).
 
-(* [exp] spreads [exp_aux] over the factors, exactly as [hl_inv] spreads
-   [hl_inv_aux]. *)
+(* [exp] spreads [exp_aux] over the group factors, exactly as [hl_ginv] spreads
+   [hl_ginv_aux]. *)
 Definition hl_exp : val := λ: "b" "e",
-  hl_mul_list (map_list (λ: "t", hl_exp_aux "t" "e") (hl_factors "b")).
+  hl_gmul_list (map_list (λ: "t", hl_exp_aux "t" "e") (hl_gfactors "b")).
 
 Definition texp : val := λ: "base" "exp", hl_exp "base" "exp".
 
@@ -239,7 +284,7 @@ Lemma twp_eq_term_op1 E (o1 o2 : term_op1) :
   ⊢ WP (eq_term_op1 (repr o1) (repr o2)) @ E
     [{ v, ⌜v = #(bool_decide (o1 = o2))⌝}].
 Proof.
-case: o1 o2 => [o1||] [o2||] /=. all: wp_lam; wp_pures => //.
+case: o1 o2 => [o1|||] [o2|||] /=. all: wp_lam; wp_pures => //.
 iApply twp_wand; first wp_apply twp_eq_key_type.
 iIntros (?) "->". iPureIntro.
 congr (# (LitBool _)). apply: bool_decide_ext.
@@ -254,14 +299,14 @@ Proof. case: o1 o2 => [] [] /=; wp_lam; wp_pures => //. Qed.
 Lemma twp_eq_term_opN E (o1 o2 : term_opN) :
   ⊢ WP (eq_term_opN (repr o1) (repr o2)) @ E
     [{ v, ⌜v = #(bool_decide (o1 = o2))⌝}].
-Proof. case: o1 o2 => [] [] /=; wp_lam; wp_pures => //. Qed.
+Proof. case: o1 o2 => [|] [|] /=; wp_lam; wp_pures => //. Qed.
 
 Lemma twp_eq_pre_term_aux E pt1 pt2 :
   ⊢ WP (eq_term (repr pt1) (repr pt2)) @ E
        [{ v, ⌜v = #(bool_decide (pt1 = pt2))⌝ }].
 Proof.
-elim: pt1 pt2 => [o1|o1 t1 IH1|o1 t11 IH1 t12 IH2|[] ts1 IHts1];
-case=> [o2|o2 t2|o2 t21 t22|[] ts2]; wp_rec; wp_pures=> //.
+elim: pt1 pt2 => [o1|o1 t1 IH1|o1 t11 IH1 t12 IH2|oN1 ts1 IHts1];
+case=> [o2|o2 t2|o2 t21 t22|oN2 ts2]; wp_rec; wp_pures=> //.
 - iApply twp_wand; first by wp_apply twp_eq_term_op0.
   iIntros (?) "->". iPureIntro; congr (# (LitBool _)).
   apply: bool_decide_ext; intuition congruence.
@@ -288,11 +333,11 @@ case=> [o2|o2 t2|o2 t21 t22|[] ts2]; wp_rec; wp_pures=> //.
   wp_pures; iPureIntro; congr (# (LitBool _)).
   rewrite bool_decide_false; congruence.
 - wp_bind (eq_term_opN _ _).
-  iApply twp_wand; first by wp_apply (twp_eq_term_opN _ ONMul ONMul).
+  iApply twp_wand; first by wp_apply (twp_eq_term_opN _ oN1 oN2).
   iIntros (?) "->".
-  have eN : bool_decide (ONMul = ONMul) = true by apply: bool_decide_eq_true_2.
-  rewrite eN; wp_pures.
-  rewrite -!repr_list_val.
+  case: (bool_decide_reflect (oN1 = oN2)) => eN; wp_pures; last first.
+    by iPureIntro; congr (# (LitBool _)); rewrite bool_decide_false; congruence.
+    rewrite -!repr_list_val.
   iApply (@twp_eq_list PreTerm.pre_term); last first.
     iPureIntro; congr (# (LitBool _)); apply: bool_decide_ext.
     by split; congruence.
@@ -328,7 +373,7 @@ Proof. by case: o1 o2 => [n1|[l1]] [n2|[l2]] /=; wp_lam; wp_pures. Qed.
 Lemma twp_leq_term_op1 E (o1 o2 : term_op1) :
   ⊢ WP (leq_term_op1 (repr o1) (repr o2)) @ E [{ v, ⌜v = #(op1_le o1 o2)⌝}].
 Proof.
-case: o1 o2 => [k1||] [k2||] /=; wp_lam; wp_pures => //.
+case: o1 o2 => [k1|||] [k2|||] /=; wp_lam; wp_pures => //.
 iApply twp_wand; first by wp_apply twp_leq_key_type.
 by iIntros (?) "->".
 Qed.
@@ -339,14 +384,14 @@ Proof. by case: o1 o2 => [] [] /=; wp_lam; wp_pures. Qed.
 
 Lemma twp_leq_term_opN E (o1 o2 : term_opN) :
   ⊢ WP (leq_term_opN (repr o1) (repr o2)) @ E [{ v, ⌜v = #(opN_le o1 o2)⌝}].
-Proof. by case: o1 o2 => [] [] /=; wp_lam; wp_pures. Qed.
+Proof. by case: o1 o2 => [|] [|] /=; wp_lam; wp_pures. Qed.
 
 Lemma twp_leq_pre_term pt1 pt2 E Ψ :
   Ψ #(bool_decide (pt_order pt1 pt2)) ⊢
   WP (leq_term (repr pt1) (repr pt2)) @ E [{ Ψ }].
 Proof.
-elim: pt1 pt2 Ψ => [o1|o1 t1 IH1|o1 t11 IH1 t12 IH2|[] ts1 IHts1];
-case => [o2|o2 t2|o2 t21 t22|[] ts2] Ψ;
+elim: pt1 pt2 Ψ => [o1|o1 t1 IH1|o1 t11 IH1 t12 IH2|oN1 ts1 IHts1];
+case => [o2|o2 t2|o2 t21 t22|oN2 ts2] Ψ;
 iIntros "post"; rewrite pt_orderE /=; wp_rec; wp_pures; try by iApply "post".
 - iApply twp_wand; first by wp_apply twp_leq_term_op0.
   by iIntros "% ->".
@@ -368,10 +413,11 @@ iIntros "post"; rewrite pt_orderE /=; wp_rec; wp_pures; try by iApply "post".
   + by iApply IH2.
   + by iApply IH1.
 wp_bind (eq_term_opN _ _).
-iApply twp_wand; first by wp_apply (twp_eq_term_opN _ ONMul ONMul).
+iApply twp_wand; first by wp_apply (twp_eq_term_opN _ oN1 oN2).
 iIntros "% ->".
-have eN : bool_decide (ONMul = ONMul) = true by apply: bool_decide_eq_true_2.
-rewrite eN; wp_pures.
+case: (bool_decide_reflect (oN1 = oN2)) => eN; wp_pures; last first.
+  iApply twp_wand; first by wp_apply twp_leq_term_opN.
+  by iIntros "% ->".
 rewrite -!repr_list_val.
 iApply twp_leq_list => //.
 - move=> x1 x2 Φ; iIntros "_ post".
@@ -392,15 +438,15 @@ Lemma twp_hl_is_inv pt E Ψ :
   Ψ #(PreTerm.is_inv pt) ⊢ WP hl_is_inv (repr pt) @ E [{ Ψ }].
 Proof.
 iIntros "HΨ"; wp_lam.
-case: pt => [o|o t|o t1 t2|[] ts] /=; wp_pures; try by iApply "HΨ".
-by case: o => [k| |] /=; wp_pures; iApply "HΨ".
+case: pt => [o|o t|o t1 t2|[|] ts] /=; wp_pures; try by iApply "HΨ".
+by case: o => [k| | |] /=; wp_pures; iApply "HΨ".
 Qed.
 
 Lemma twp_hl_is_exp pt E Ψ :
   Ψ #(PreTerm.is_exp pt) ⊢ WP hl_is_exp (repr pt) @ E [{ Ψ }].
 Proof.
 iIntros "HΨ"; wp_lam.
-case: pt => [o|o t|o t1 t2|[] ts]; try by (wp_pures; iApply "HΨ").
+case: pt => [o|o t|o t1 t2|[|] ts]; try by (wp_pures; iApply "HΨ").
 all: by case: o; wp_pures; iApply "HΨ".
 Qed.
 
@@ -408,14 +454,29 @@ Lemma twp_hl_is_mul pt E Ψ :
   Ψ #(PreTerm.is_mul pt) ⊢ WP hl_is_mul (repr pt) @ E [{ Ψ }].
 Proof.
 iIntros "HΨ"; wp_lam.
-by case: pt => [o|o t|o t1 t2|[] ts] /=; wp_pures; iApply "HΨ".
+by case: pt => [o|o t|o t1 t2|[|] ts] /=; wp_pures; iApply "HΨ".
+Qed.
+
+Lemma twp_hl_is_ginv pt E Ψ :
+  Ψ #(PreTerm.is_ginv pt) ⊢ WP hl_is_ginv (repr pt) @ E [{ Ψ }].
+Proof.
+iIntros "HΨ"; wp_lam.
+case: pt => [o|o t|o t1 t2|[|] ts] /=; wp_pures; try by iApply "HΨ".
+by case: o => [k| | |] /=; wp_pures; iApply "HΨ".
+Qed.
+
+Lemma twp_hl_is_gmul pt E Ψ :
+  Ψ #(PreTerm.is_gmul pt) ⊢ WP hl_is_gmul (repr pt) @ E [{ Ψ }].
+Proof.
+iIntros "HΨ"; wp_lam.
+by case: pt => [o|o t|o t1 t2|[|] ts] /=; wp_pures; iApply "HΨ".
 Qed.
 
 Lemma twp_hl_is_nonce pt E Ψ :
   Ψ #(PreTerm.is_nonce pt) ⊢ WP hl_is_nonce (repr pt) @ E [{ Ψ }].
 Proof.
 iIntros "HΨ"; wp_lam.
-case: pt => [o|o t|o t1 t2|[] ts]; try by (wp_pures; iApply "HΨ").
+case: pt => [o|o t|o t1 t2|[|] ts]; try by (wp_pures; iApply "HΨ").
 all: by case: o => [n|a]; wp_pures; iApply "HΨ".
 Qed.
 
@@ -426,7 +487,7 @@ Lemma twp_hl_base pt E Ψ :
 Proof.
 iIntros "HΨ"; wp_lam.
 wp_apply twp_hl_is_exp.
-case: pt => [o|o t|o t1 t2|[] ts]; try by (wp_pures; iApply "HΨ").
+case: pt => [o|o t|o t1 t2|[|] ts]; try by (wp_pures; iApply "HΨ").
 all: by case: o; wp_pures; iApply "HΨ".
 Qed.
 
@@ -438,7 +499,7 @@ have one : repr (PreTerm.PTMul []) = hl_one.
 iIntros "HΨ"; wp_lam.
 wp_apply twp_hl_is_exp.
 rewrite /PreTerm.expo -?one.
-case: pt => [o|o t|o t1 t2|[] ts]; try by (wp_pures; rewrite -?one; iApply "HΨ").
+case: pt => [o|o t|o t1 t2|[|] ts]; try by (wp_pures; rewrite -?one; iApply "HΨ").
 all: by case: o; wp_pures; rewrite -?one; iApply "HΨ".
 Qed.
 
@@ -451,8 +512,22 @@ have reprS : forall pt' : PreTerm.pre_term,
 iIntros "HΨ"; wp_lam.
 wp_apply twp_hl_is_mul.
 rewrite /PreTerm.factors.
-case: pt => [o|o t|o t1 t2|[] ts]; wp_pures.
-1-3: rewrite /CONS; wp_pures; iEval (rewrite reprS /=) in "HΨ"; by iApply "HΨ".
+case: pt => [o|o t|o t1 t2|[|] ts]; wp_pures.
+1-3,5: rewrite /CONS; wp_pures; iEval (rewrite reprS /=) in "HΨ"; by iApply "HΨ".
+by rewrite -repr_list_val; iApply "HΨ".
+Qed.
+
+Lemma twp_hl_gfactors pt E Ψ :
+  Ψ (repr (PreTerm.gfactors pt)) ⊢ WP hl_gfactors (repr pt) @ E [{ Ψ }].
+Proof.
+have reprS : forall pt' : PreTerm.pre_term,
+    repr [pt'] = InjRV (repr pt', InjLV #()).
+  by move=> pt'; rewrite repr_list_unseal.
+iIntros "HΨ"; wp_lam.
+wp_apply twp_hl_is_gmul.
+rewrite /PreTerm.gfactors.
+case: pt => [o|o t|o t1 t2|[|] ts]; wp_pures.
+1-4: rewrite /CONS; wp_pures; iEval (rewrite reprS /=) in "HΨ"; by iApply "HΨ".
 by rewrite -repr_list_val; iApply "HΨ".
 Qed.
 
@@ -463,13 +538,36 @@ Lemma twp_hl_inv_aux pt E Ψ :
 Proof.
 iIntros "HΨ"; wp_lam.
 wp_apply twp_hl_is_inv.
-case: pt => [o|o t|o t1 t2|[] ts]; try by (wp_pures; iApply "HΨ").
-all: by case: o => [k| |]; wp_pures; iApply "HΨ".
+case: pt => [o|o t|o t1 t2|[|] ts]; try by (wp_pures; iApply "HΨ").
+all: by case: o => [k| | |]; wp_pures; iApply "HΨ".
 Qed.
 
 Lemma wp_hl_inv_aux E pt Ψ :
   Ψ (repr (PreTerm.inv_aux pt)) ⊢ WP hl_inv_aux (repr pt) @ E {{ Ψ }}.
 Proof. iIntros "HΨ"; iApply twp_wp; by wp_apply twp_hl_inv_aux. Qed.
+
+Lemma twp_hl_ginv_aux pt E Ψ :
+  Ψ (repr (PreTerm.ginv_aux pt)) ⊢ WP hl_ginv_aux (repr pt) @ E [{ Ψ }].
+Proof.
+iIntros "HΨ"; wp_lam.
+wp_apply twp_hl_is_ginv.
+case: pt => [o|o t|o t1 t2|[|] ts]; try by (wp_pures; iApply "HΨ").
+all: by case: o => [k| | |]; wp_pures; iApply "HΨ".
+Qed.
+
+Lemma wp_hl_ginv_aux E pt Ψ :
+  Ψ (repr (PreTerm.ginv_aux pt)) ⊢ WP hl_ginv_aux (repr pt) @ E {{ Ψ }}.
+Proof. iIntros "HΨ"; iApply twp_wp; by wp_apply twp_hl_ginv_aux. Qed.
+
+Lemma twp_hl_gmul_aux E (ts : list PreTerm.pre_term) Ψ :
+  Ψ (repr (PreTerm.gmul_aux ts)) ⊢ WP hl_gmul_aux (repr ts) @ E [{ Ψ }].
+Proof.
+iIntros "HΨ"; rewrite /hl_gmul_aux /hl_gone; wp_lam.
+case: ts => [|t [|u ts]]; rewrite {1}repr_list_unseal /=; wp_pures.
+- iEval (rewrite repr_list_unseal /=) in "HΨ"; by iApply "HΨ".
+- by iApply "HΨ".
+- by rewrite [repr_list (t :: u :: ts)]repr_list_val; iApply "HΨ".
+Qed.
 
 Lemma twp_hl_mul_aux E (ts : list PreTerm.pre_term) Ψ :
   Ψ (repr (PreTerm.mul_aux ts)) ⊢ WP hl_mul_aux (repr ts) @ E [{ Ψ }].
@@ -494,6 +592,80 @@ wp_apply (twp_foldr_list (λ (t : PreTerm.pre_term) (acc : list PreTerm.pre_term
   by iApply "HΦ".
 iIntros "_".
 by iApply "HΨ".
+Qed.
+
+Lemma twp_hl_all_gfactors E (ts : list PreTerm.pre_term) Ψ :
+  Ψ (repr (mbind PreTerm.gfactors ts)) ⊢ WP hl_all_gfactors (repr ts) @ E [{ Ψ }].
+Proof.
+iIntros "HΨ"; wp_lam.
+wp_pures; wp_apply twp_nil.
+wp_apply (twp_foldr_list (λ (t : PreTerm.pre_term) (acc : list PreTerm.pre_term),
+                           PreTerm.gfactors t ++ acc)) => //.
+  iIntros "%b %a %Φ _ HΦ"; wp_pures.
+  wp_apply twp_hl_gfactors.
+  wp_apply twp_append_lists.
+  by iApply "HΦ".
+iIntros "_".
+by iApply "HΨ".
+Qed.
+
+Lemma twp_hl_normalize_gfactors E (ts : list PreTerm.pre_term) Ψ :
+  Ψ (repr (PreTerm.normalize_gfactors ts)) ⊢
+  WP hl_normalize_gfactors (repr ts) @ E [{ Ψ }].
+Proof.
+iIntros "HΨ"; wp_lam.
+wp_apply twp_hl_all_gfactors.
+wp_apply (twp_sms_to pt_order PreTerm.ginv_aux eq_term hl_ginv_aux leq_term
+            twp_eq_pre_term twp_hl_ginv_aux twp_leq_pre_term).
+by iApply "HΨ".
+Qed.
+
+Lemma twp_hl_gmul_list E (ts : list PreTerm.pre_term) Ψ :
+  Ψ (repr (PreTerm.gmul ts)) ⊢ WP hl_gmul_list (repr ts) @ E [{ Ψ }].
+Proof.
+iIntros "HΨ"; wp_lam.
+wp_apply twp_hl_normalize_gfactors.
+wp_apply twp_hl_gmul_aux.
+by iApply "HΨ".
+Qed.
+
+Lemma twp_hl_gmul E pt1 pt2 Ψ :
+  Ψ (repr (PreTerm.gmul [pt1; pt2])) ⊢
+  WP hl_gmul (repr pt1) (repr pt2) @ E [{ Ψ }].
+Proof.
+iIntros "HΨ"; wp_lam; wp_pures.
+wp_apply twp_nil.
+wp_apply twp_cons.
+wp_apply twp_cons.
+wp_apply twp_hl_gmul_list.
+by iApply "HΨ".
+Qed.
+
+Lemma twp_hl_ginv E pt Ψ :
+  Ψ (repr (PreTerm.ginv pt)) ⊢ WP hl_ginv (repr pt) @ E [{ Ψ }].
+Proof.
+have invS : forall pt' : PreTerm.pre_term,
+    [[{ True }]] hl_ginv_aux (repr pt') @ E
+    [[{ RET repr (PreTerm.ginv_aux pt'); True }]].
+  by iIntros "%pt' %Φ _ HΦ"; wp_apply twp_hl_ginv_aux; iApply "HΦ".
+have mapE : forall T (f : PreTerm.pre_term -> T) (l : list PreTerm.pre_term),
+    map f l = f <$> l.
+  by move=> T f; elim=> [//|x l IH] /=; rewrite IH.
+have invE : PreTerm.is_gmul pt = true ->
+    PreTerm.ginv pt = PreTerm.gmul (PreTerm.ginv_aux <$> PreTerm.gfactors pt).
+  by case: pt => [o|o t|o t1 t2|[|] ts].
+iIntros "HΨ"; wp_lam.
+wp_apply twp_hl_is_gmul.
+case Em: (PreTerm.is_gmul pt); wp_pures.
+- rewrite (invE Em).
+  wp_apply twp_hl_gfactors.
+  wp_apply (twp_map_list PreTerm.ginv_aux hl_ginv_aux) => //.
+    by apply/Forall_forall => x _; exact: invS.
+  iIntros "_"; rewrite mapE.
+  wp_apply twp_hl_gmul_list.
+  by iApply "HΨ".
+- rewrite PreTerm.ginv_Ngmul; last by rewrite Em.
+  by wp_apply twp_hl_ginv_aux; iApply "HΨ".
 Qed.
 
 Lemma twp_hl_normalize_factors E (ts : list PreTerm.pre_term) Ψ :
@@ -538,7 +710,7 @@ have mapE : forall T (f : PreTerm.pre_term -> T) (l : list PreTerm.pre_term),
   by move=> T f; elim=> [//|x l IH] /=; rewrite IH.
 have invE : PreTerm.is_mul pt = true ->
     PreTerm.inv pt = PreTerm.mul (PreTerm.inv_aux <$> PreTerm.factors pt).
-  by case: pt => [o|o t|o t1 t2|[] ts].
+  by case: pt => [o|o t|o t1 t2|[|] ts].
 iIntros "HΨ"; wp_lam.
 wp_apply twp_hl_is_mul.
 case Em: (PreTerm.is_mul pt); wp_pures.
@@ -585,14 +757,14 @@ Lemma twp_hl_exp_aux E (b e : PreTerm.pre_term) Ψ :
   Ψ (repr (PreTerm.exp_aux b e)) ⊢ WP hl_exp_aux (repr b) (repr e) @ E [{ Ψ }].
 Proof.
 iIntros "HΨ"; wp_lam; wp_pures.
-wp_apply twp_hl_is_inv.
-case Ei: (PreTerm.is_inv b); wp_pures.
-- wp_apply twp_hl_inv_aux; wp_pures.
+wp_apply twp_hl_is_ginv.
+case Ei: (PreTerm.is_ginv b); wp_pures.
+- wp_apply twp_hl_ginv_aux; wp_pures.
   wp_apply twp_hl_exp_aux_body.
-  wp_apply twp_hl_inv_aux.
-  by case: b Ei => [o|[k| |] u|o c d|[] us] //= _; iApply "HΨ".
+  wp_apply twp_hl_ginv_aux.
+  by case: b Ei => [o|[k| | |] u|o c d|[|] us] //= _; iApply "HΨ".
 - wp_apply twp_hl_exp_aux_body.
-  rewrite PreTerm.exp_aux_Ninv; last by rewrite Ei.
+  rewrite PreTerm.exp_aux_Nginv; last by rewrite Ei.
   by iApply "HΨ".
 Qed.
 
@@ -608,11 +780,11 @@ have mapE : forall T (f : PreTerm.pre_term -> T) (l : list PreTerm.pre_term),
     map f l = f <$> l.
   by move=> T f; elim=> [//|x l IH] /=; rewrite IH.
 iIntros "HΨ"; wp_lam; wp_pures.
-wp_apply twp_hl_factors; wp_pures.
+wp_apply twp_hl_gfactors; wp_pures.
 wp_apply (twp_map_list (fun t => PreTerm.exp_aux t e)) => //.
   by apply/Forall_forall => x _; exact: expS.
 iIntros "_"; rewrite mapE.
-wp_apply twp_hl_mul_list.
+wp_apply twp_hl_gmul_list.
 by iApply "HΨ".
 Qed.
 
