cryptis/core/public.v
@@ -88,7 +88,7 @@ Definition exp_pred0_pre Plater P DH ts : iProp :=
     [∗ list] t ∈ ts', Plater t) ∨
   P ts.1 ∨
   ∃ t2' t, ⌜ts.2 = TExp t2' t⌝ ∗ ⌜negb (is_mul t)⌝ ∗
-  ⌜negb (is_mul t2')⌝ ∗ ⌜negb (is_inv t2')⌝ ∗ ⌜TInv t ∉ exps t2'⌝ ∗
+  ⌜negb (is_gmul t2')⌝ ∗ ⌜negb (is_ginv t2')⌝ ∗ ⌜TInv t ∉ exps t2'⌝ ∗
   DH (ts.1, t2') ∗ DH (t, ts.2).
 
 Local Instance exp_pred0_pre_mono Plater P :
@@ -118,7 +118,7 @@ Lemma exp_pred0_unfold Plater P ts :
     [∗ list] t ∈ ts', Plater t) ∨
   P ts.1 ∨
   ∃ t2' t, ⌜ts.2 = TExp t2' t⌝ ∗ ⌜negb (is_mul t)⌝ ∗
-  ⌜negb (is_mul t2')⌝ ∗ ⌜negb (is_inv t2')⌝ ∗ ⌜TInv t ∉ exps t2'⌝ ∗
+  ⌜negb (is_gmul t2')⌝ ∗ ⌜negb (is_ginv t2')⌝ ∗ ⌜TInv t ∉ exps t2'⌝ ∗
   exp_pred0 Plater P (ts.1, t2') ∗ exp_pred0 Plater P (t, ts.2).
 Proof. by rewrite exp_pred0_unseal /exp_pred0_def least_fixpoint_unfold. Qed.
 
@@ -375,13 +375,49 @@ Qed.
 Lemma is_inv_Nmul t : is_inv t -> is_mul t = false.
 Proof.
 rewrite is_inv_unfold is_mul_unfold.
-by case: (unfold_term t) => [?|[?| |]?|???|[] ?] //=.
+by case: (unfold_term t) => [?|[?| | |]?|???|[|] ?] //=.
 Qed.
 
 Lemma is_inv_Nexp t : is_inv t -> is_exp t = false.
 Proof.
 rewrite is_inv_unfold is_exp_unfold.
-by case: (unfold_term t) => [?|[?| |]?|???|[] ?] //=.
+by case: (unfold_term t) => [?|[?| | |]?|???|[|] ?] //=.
+Qed.
+
+Lemma is_inv_Ngmul t : is_inv t -> is_gmul t = false.
+Proof.
+rewrite is_inv_unfold is_gmul_unfold.
+by case: (unfold_term t) => [?|[?| | |]?|???|[|] ?] //=.
+Qed.
+
+Lemma is_ginv_Nmul t : is_ginv t -> is_mul t = false.
+Proof.
+rewrite is_ginv_unfold is_mul_unfold.
+by case: (unfold_term t) => [?|[?| | |]?|???|[|] ?] //=.
+Qed.
+
+Lemma is_ginv_Ngmul' t : is_ginv t -> is_gmul t = false.
+Proof.
+rewrite is_ginv_unfold is_gmul_unfold.
+by case: (unfold_term t) => [?|[?| | |]?|???|[|] ?] //=.
+Qed.
+
+Lemma is_inv_Nginv t : is_inv t -> is_ginv t = false.
+Proof.
+rewrite is_inv_unfold is_ginv_unfold.
+by case: (unfold_term t) => [?|[?| | |]?|???|[|] ?] //=.
+Qed.
+
+Lemma is_ginv_Ninv t : is_ginv t -> is_inv t = false.
+Proof.
+rewrite is_ginv_unfold is_inv_unfold.
+by case: (unfold_term t) => [?|[?| | |]?|???|[|] ?] //=.
+Qed.
+
+Lemma is_ginv_Nexp t : is_ginv t -> is_exp t = false.
+Proof.
+rewrite is_ginv_unfold is_exp_unfold.
+by case: (unfold_term t) => [?|[?| | |]?|???|[|] ?] //=.
 Qed.
 
 Inductive decompose (T : gset term) (t : term) : Prop :=
@@ -395,7 +431,9 @@ Inductive decompose (T : gset term) (t : term) : Prop :=
 
 | DHash t' of T = {[t']} & t = THash t'
 
-| DInv t' of T = {[t']} & ¬ is_inv t' & is_inv t & t = TInv t'.
+| DInv t' of T = {[t']} & ¬ is_inv t' & is_inv t & t = TInv t'
+
+| DGInv t' of T = {[t']} & ¬ is_ginv t' & is_ginv t & t = TGInv t'.
 
 Lemma decompose_tsize T t t' : decompose T t → t' ∈ T → tsize t' < tsize t.
 Proof.
@@ -404,30 +442,46 @@ case; try by move =>> -> -> //;
           move => /elem_of_singleton ->;
           rewrite [tsize (_ _)]tsize_eq;
           lia.
-move => t'' -> Ninv inv_t E; rewrite E in inv_t *.
-move => /elem_of_singleton ->.
-have NmI : negb (is_mul (TInv t'')) by rewrite (is_inv_Nmul inv_t).
-have Nm : negb (is_mul t'') by move: NmI; rewrite is_mul_TInv.
-have Ninv' : negb (is_inv t'') by apply/negb_True.
-rewrite (tsize_TInv t'' Nm Ninv'); lia.
+- move => t'' -> Ninv inv_t E; rewrite E in inv_t *.
+  move => /elem_of_singleton ->.
+  have NmI : negb (is_mul (TInv t'')) by rewrite (is_inv_Nmul inv_t).
+  have Nm : negb (is_mul t'') by move: NmI; rewrite is_mul_TInv.
+  have Ninv' : negb (is_inv t'') by apply/negb_True.
+  rewrite (tsize_TInv t'' Nm Ninv'); lia.
+- move => t'' -> Ninv inv_t E; rewrite E in inv_t *.
+  move => /elem_of_singleton ->.
+  have NmI : negb (is_gmul (TGInv t'')) by rewrite (is_ginv_Ngmul' inv_t).
+  have Nm : negb (is_gmul t'') by move: NmI; rewrite is_gmul_TGInv.
+  have Ninv' : negb (is_ginv t'') by apply/negb_True.
+  rewrite (tsize_TGInv t'' Nm Ninv'); lia.
 Qed.
 
 Lemma decompose_is_mul T t : decompose T t → is_mul t = false.
 Proof.
 case => *; subst => //=.
-by apply: is_inv_Nmul.
+- by apply: is_inv_Nmul.
+- by apply: is_ginv_Nmul.
+Qed.
+
+Lemma decompose_is_gmul T t : decompose T t → is_gmul t = false.
+Proof.
+case => *; subst => //=.
+- by apply: is_inv_Ngmul.
+- by apply: is_ginv_Ngmul'.
 Qed.
 
 Lemma decompose_is_exp T t : decompose T t → is_exp t = false.
 Proof.
 case => *; subst => //=.
-by apply: is_inv_Nexp.
+- by apply: is_inv_Nexp.
+- by apply: is_ginv_Nexp.
 Qed.
 
 Definition public_pre_aux Plater P t : iProp :=
   minted t ∧ (
    (∃ T, ⌜decompose T t⌝ ∧ [∗ set] t' ∈ T, P t')
    ∨ (⌜is_mul t⌝ ∧ [∗ list] t' ∈ factors t, P t')
+   ∨ (⌜is_gmul t⌝ ∧ [∗ list] t' ∈ gfactors t, P t')
    ∨ (⌜is_exp t⌝ ∧
       [∗ list] t' ∈ exps t,
         ⌜negb (is_mul (TInv t'))⌝ ∧
@@ -462,7 +516,7 @@ Lemma public_pre_aux_wf Plater :
 Proof.
 move => P1 P2 {}t HP; rewrite /public_pre_aux.
 f_equiv.
-f_equiv; last (f_equiv; last f_equiv).
+f_equiv; last (f_equiv; last (f_equiv; last f_equiv)).
 - f_equiv => T; apply: and_proper_L => T_t.
   apply: big_sepS_proper => t' T_t'.
   by move: (decompose_tsize T_t T_t') => ?; eauto.
@@ -470,6 +524,10 @@ f_equiv; last (f_equiv; last f_equiv).
   apply: big_sepL_proper => _ t' /(list_elem_of_lookup_2 _ _ _) t'_in.
   apply: HP.
   exact: (tsize_factors_lt t' t mul_t t'_in).
+- apply: and_proper_L => mul_t.
+  apply: big_sepL_proper => _ t' /(list_elem_of_lookup_2 _ _ _) t'_in.
+  apply: HP.
+  exact: (tsize_gfactors_lt t' t mul_t t'_in).
 - apply: and_proper_L => exp_t.
   apply: big_sepL_proper => _ t' /(list_elem_of_lookup_2 _ _ _) t'_in.
   apply: and_proper_L => Nm.
@@ -497,7 +555,7 @@ Lemma public_pre_aux_persistent Plater P :
   □ (∀ t, P t -∗ <pers> P t) -∗
   ∀ t, public_pre_aux Plater P t -∗ <pers> public_pre_aux Plater P t.
 Proof.
-iIntros "#wand1 #wand2 %t [#m [H | [H | [H | H]]]]"; iSplit => //.
+iIntros "#wand1 #wand2 %t [#m [H | [H | [H | [H | H]]]]]"; iSplit => //.
 - iDestruct "H" as (T ?) "H"; iLeft; iExists T; iSplit; eauto.
   iAssert ([∗ set] t' ∈ T, <pers> P t')%I as "{H} #H".
   { iApply (big_sepS_impl with "H"); iIntros "!> %t' _".
@@ -509,6 +567,11 @@ iIntros "#wand1 #wand2 %t [#m [H | [H | [H | H]]]]"; iSplit => //.
     by iApply "wand2". }
   by iModIntro; iSplit => //; iApply (big_sepL_impl with "H"); eauto.
 - iDestruct "H" as "(% & H)"; iRight; iRight; iLeft.
+  iAssert ([∗ list] t' ∈ gfactors t, <pers> P t')%I as "{H} #H".
+  { iApply (big_sepL_impl with "H"); iIntros "!> %k %t' _".
+    by iApply "wand2". }
+  by iModIntro; iSplit => //; iApply (big_sepL_impl with "H"); eauto.
+- iDestruct "H" as "(% & H)"; iRight; iRight; iRight; iLeft.
   iAssert ([∗ list] t' ∈ exps t,
     ⌜negb (is_mul (TInv t'))⌝ ∧
     <pers> exp_pred0 Plater P (t', t) ∧
@@ -521,7 +584,7 @@ iIntros "#wand1 #wand2 %t [#m [H | [H | [H | H]]]]"; iSplit => //.
     by iModIntro; iApply (exp_pred0_wand with "[] [] dh"); iIntros "!> % #?". }
   iModIntro; iSplit => //.
   by iApply (big_sepL_impl with "H"); iIntros "!> % % _ [% [#? #?]]"; eauto.
-- iRight; iRight; iRight; case: t; by move=> *; iPoseProof "H" as "#H".
+- iRight; iRight; iRight; iRight; case: t; by move=> *; iPoseProof "H" as "#H".
 Qed.
 
 Lemma public_pre_unfold Plater t :
@@ -576,6 +639,7 @@ Lemma public_eq t :
   minted t ∧ (
       (∃ T, ⌜decompose T t⌝ ∧ [∗ set] t' ∈ T, public t')
      ∨ (⌜is_mul t⌝ ∧ [∗ list] t' ∈ factors t, public t')
+     ∨ (⌜is_gmul t⌝ ∧ [∗ list] t' ∈ gfactors t, public t')
      ∨ (⌜is_exp t⌝ ∧
         [∗ list] t' ∈ exps t,
           ⌜negb (is_mul (TInv t'))⌝ ∧
@@ -640,7 +704,7 @@ by iApply (@exp_pred_intro1_gen t1 t2 [] atom0 hexps).
 Qed.
 
 Lemma exp_pred_intro2 t t1 t2 :
-  negb (is_mul t) -> negb (is_mul t2) -> negb (is_inv t2) ->
+  negb (is_mul t) -> negb (is_gmul t2) -> negb (is_ginv t2) ->
   TInv t ∉ exps t2 →
   exp_pred t1 t2 -∗ exp_pred t (TExp t2 t) -∗ exp_pred t1 (TExp t2 t).
 Proof.
@@ -662,7 +726,7 @@ Lemma exp_pred_ind (φ : term → term → iProp) :
     ([∗ list] t ∈ ts, ▷ public t) -∗
     exp_pred_base t1 (TExpN t2 ts) -∗ φ t1 t2) -∗
   (□ ∀ t t1 t2, ⌜negb (is_mul t)⌝ -∗
-                ⌜negb (is_mul t2)⌝ -∗ ⌜negb (is_inv t2)⌝ -∗
+                ⌜negb (is_gmul t2)⌝ -∗ ⌜negb (is_ginv t2)⌝ -∗
                 ⌜TInv t ∉ exps t2⌝ -∗
                 exp_pred t1 t2 -∗ □ φ t1 t2 -∗
                 exp_pred t (TExp t2 t) -∗ □ φ t (TExp t2 t) -∗
@@ -698,7 +762,7 @@ iApply exp_pred_ind; eauto 10.
 - iIntros "!> %ts %t1 %t2 %atom_ts %ts_t2 #p_ts #base %ts' %t1_ts' %ts'_t2".
   (* [t1 ∈ ts' ⊆ exps t2] makes [t2] an exponential, hence atom-headed *)
   have xt2 := is_exp_of_exps (ts'_t2 _ t1_ts').
-  have Nm2 := is_exp_Nmul _ xt2; have Ni2 := is_exp_Ninv _ xt2.
+  have Nm2 := is_exp_Ngmul _ xt2; have Ni2 := is_exp_Nginv _ xt2.
   iExists t1; iSplit=> //; iRight; iExists (TExpN t2 ts).
   have baseE : base (TExpN t2 ts) = base t2.
     by rewrite /TExpN (base_TExp _ _ Nm2 Ni2).
@@ -758,7 +822,7 @@ Proof.
 apply: (anti_symm _); iIntros "#Ht" => //.
 - rewrite public_eq minted_TPair.
   iDestruct "Ht" as "([Ht1 Ht2] & publ)".
-  iDestruct "publ" as "[publ | [(? & _) | [(? & _) | publ]]]" => //=.
+  iDestruct "publ" as "[publ | [(? & _) | [(? & _) | [(? & _) | publ]]]]" => //=.
   iDestruct "publ" as (T) "[%dec publ]".
   case: dec => //= {}t1 {}t2 -> [-> ->].
   by rewrite big_sepS_union_pers !big_sepS_singleton.
@@ -776,7 +840,7 @@ Proof.
 apply: (anti_symm _); iIntros "Ht".
 - rewrite public_eq; iDestruct "Ht" as "[? Ht]".
   rewrite minted_TNonce. iFrame.
-  iDestruct "Ht" as "[publ | [ (? & _) | [ (? & _) | ? ] ]]" => //.
+  iDestruct "Ht" as "[publ | [ (? & _) | [ (? & _) | [ (? & _) | ? ] ] ]]" => //.
   iDestruct "publ" as (T) "[%dec _]".
   by case: dec.
 - rewrite public_eq minted_TNonce /pnonce.
@@ -798,13 +862,17 @@ have Nm' : negb (is_mul t) := Nm.
 have Ninv' : negb (is_inv t) := Ninv.
 apply: anti_symm.
 - rewrite [public (TInv t)]public_eq minted_TInv.
-  iIntros "[_ [dec | [ [%mul _] | [ [%exp _] | Hstr]]]]".
+  iIntros "[_ [dec | [ [%mul _] | [ [%gmul _] | [ [%exp _] | Hstr]]]]]".
   + iDestruct "dec" as (T) "[%d publ]".
     have invI : is_inv (TInv t) by rewrite (is_inv_TInv t Nm').
-    case: d => [n eT et|t1 t2 eT et|kt t0 eT et|k t0 eT et|t0 eT et|s eT Ns Hi et];
+    case: d => [n eT et|t1 t2 eT et|kt t0 eT et|k t0 eT et|t0 eT et
+               |s eT Ns Hi et|s eT Ns Hi et];
       try by move: invI; rewrite et.
-    move: et => /TInv_inj ->; rewrite eT big_sepS_singleton. by [].
+    * move: et => /TInv_inj ->; rewrite eT big_sepS_singleton. by [].
+    * by move: Hi; rewrite (is_inv_Nginv invI).
   + by move: Nm'; rewrite -is_mul_TInv (proj2 (is_trueP _) mul).
+  + have invI : is_inv (TInv t) by rewrite (is_inv_TInv t Nm').
+    by move: (is_inv_Ngmul invI); rewrite (proj2 (is_trueP _) gmul).
   + by move: (is_exp_TInv t Nm' Ninv'); rewrite (proj2 (is_trueP _) exp).
   + have invI : is_inv (TInv t) by rewrite (is_inv_TInv t Nm').
     iRevert "Hstr".
@@ -824,12 +892,14 @@ Lemma public_TMulN t :
   public t ⊢ [∗ list] t' ∈ factors t, public t'.
 Proof.
 move=> mul_t; rewrite public_eq.
-iIntros "[_ [publ | [ [_ Hfs] | [ (%exp_t & _) | Hstr ]]]]".
+iIntros "[_ [publ | [ [_ Hfs] | [ [%gmul_t _] | [ (%exp_t & _) | Hstr ]]]]]".
 - iDestruct "publ" as (T) "[%dec _]".
   by move: mul_t; rewrite (decompose_is_mul dec).
 - by iApply "Hfs".
+- by move: mul_t gmul_t;
+     rewrite is_mul_unfold is_gmul_unfold; case: (unfold_term t) => [|||[|] ?].
 - by move: mul_t exp_t;
-     rewrite is_mul_unfold is_exp_unfold; case: (unfold_term t) => [|||[] ?].
+     rewrite is_mul_unfold is_exp_unfold; case: (unfold_term t) => [|||[|] ?].
 - by case: (t) mul_t => // *; iDestruct "Hstr" as "[]".
 Qed.
 
@@ -850,6 +920,96 @@ case Emul: (is_mul t); last first.
     by iRight; iLeft; iSplit.
 Qed.
 
+(** The group product and the group inverse get exactly the treatment the
+    exponent product and inverse get: [public] of a group product is the
+    conjunction over its group factors, and [public (TGInv t) ⊣⊢ public t]. *)
+
+Lemma public_TGInv_Ngmul t : negb (is_gmul t) → public (TGInv t) ⊣⊢ public t.
+Proof.
+wlog: t / negb (is_ginv t).
+{ move => H Nm.
+  case Einv: (is_ginv t); last by apply: H => //; rewrite Einv.
+  have Nm' : negb (is_gmul t) := Nm.
+  have NmI : negb (is_gmul (TGInv t)) by rewrite is_gmul_TGInv.
+  have NinvI : negb (is_ginv (TGInv t)) by rewrite (is_ginv_TGInv t Nm') Einv.
+  by move: (H (TGInv t) NinvI NmI);
+     rewrite TGInvK => <-. }
+move => Ninv Nm.
+have Nm' : negb (is_gmul t) := Nm.
+have Ninv' : negb (is_ginv t) := Ninv.
+apply: anti_symm.
+- rewrite [public (TGInv t)]public_eq minted_TGInv.
+  iIntros "[_ [dec | [ [%mul _] | [ [%gmul _] | [ [%exp _] | Hstr]]]]]".
+  + iDestruct "dec" as (T) "[%d publ]".
+    have invI : is_ginv (TGInv t) by rewrite (is_ginv_TGInv t Nm').
+    case: d => [n eT et|t1 t2 eT et|kt t0 eT et|k t0 eT et|t0 eT et
+               |s eT Ns Hi et|s eT Ns Hi et];
+      try by move: invI; rewrite et.
+    * by move: Hi; rewrite (is_ginv_Ninv invI).
+    * move: et => /TGInv_inj ->; rewrite eT big_sepS_singleton. by [].
+  + have invI : is_ginv (TGInv t) by rewrite (is_ginv_TGInv t Nm').
+    by move: (is_ginv_Nmul invI); rewrite (proj2 (is_trueP _) mul).
+  + by move: Nm'; rewrite -is_gmul_TGInv (proj2 (is_trueP _) gmul).
+  + by move: (is_exp_TGInv t Nm' Ninv'); rewrite (proj2 (is_trueP _) exp).
+  + have invI : is_ginv (TGInv t) by rewrite (is_ginv_TGInv t Nm').
+    iRevert "Hstr".
+    case E: (TGInv t) invI => [n|t1 t2|a|kt k|k m|h|pt wf nf] //= _;
+      by iIntros "[]".
+- iIntros "#publ".
+  rewrite [public (TGInv t)]public_eq minted_TGInv.
+  iSplit; first by iApply public_minted.
+  iLeft. iExists {[t]}. iSplit; last by rewrite big_sepS_singleton.
+  iPureIntro. apply: DGInv => //.
+  + by move=> H; move: Ninv'; rewrite (proj2 (is_trueP _) H).
+  + by rewrite (is_ginv_TGInv t Nm').
+Qed.
+
+Lemma public_TGMulN t :
+  is_gmul t ->
+  public t ⊢ [∗ list] t' ∈ gfactors t, public t'.
+Proof.
+move=> mul_t; rewrite public_eq.
+iIntros "[_ [publ | [ [%mul_t' _] | [ [_ Hfs] | [ (%exp_t & _) | Hstr ]]]]]".
+- iDestruct "publ" as (T) "[%dec _]".
+  by move: mul_t; rewrite (decompose_is_gmul dec).
+- by move: mul_t mul_t';
+     rewrite is_mul_unfold is_gmul_unfold; case: (unfold_term t) => [|||[|] ?].
+- by iApply "Hfs".
+- by move: mul_t exp_t;
+     rewrite is_gmul_unfold is_exp_unfold; case: (unfold_term t) => [|||[|] ?].
+- by case: (t) mul_t => // *; iDestruct "Hstr" as "[]".
+Qed.
+
+Lemma public_gfactors t :
+  public t ⊣⊢ minted t ∧ [∗ list] t' ∈ gfactors t, public t'.
+Proof.
+case Emul: (is_gmul t); last first.
+- rewrite gfactors_Ngmul; last by rewrite Emul.
+  rewrite big_sepL_singleton.
+  apply: (anti_symm _).
+  + by iIntros "#p"; iSplit; first iApply public_minted.
+  + by iIntros "[_ $]".
+- have mulI : is_gmul t by rewrite Emul.
+  apply: (anti_symm _).
+  + iIntros "#p"; iSplit; first by iApply public_minted.
+    by iApply (public_TGMulN mulI with "p").
+  + iIntros "[#m #fs]"; rewrite [public t]public_eq; iSplit => //.
+    by iRight; iRight; iLeft; iSplit.
+Qed.
+
+Lemma public_TGInv t : public (TGInv t) ⊣⊢ public t.
+Proof.
+have key : forall l, ginvs_canceled l ->
+  ([∗ list] u ∈ map TGInv l, public u) ⊣⊢ [∗ list] u ∈ l, public u.
+{ elim => [//|u us IH] /ginvs_canceled_cons [_ [Nmu atom]].
+  rewrite (_ : map TGInv (u :: us) = TGInv u :: map TGInv us) //.
+  by rewrite !big_sepL_cons (public_TGInv_Ngmul Nmu) (IH atom). }
+rewrite (public_gfactors (TGInv t)) (public_gfactors t) minted_TGInv.
+f_equiv.
+setoid_rewrite (gfactors_TGInv t).
+by rewrite (key _ (ginvs_canceled_gfactors t)).
+Qed.
+
 Lemma public_TInv t : public (TInv t) ⊣⊢ public t.
 Proof.
 have key : forall l, invs_canceled l ->
@@ -868,7 +1028,7 @@ Lemma public_TKey kt t :
 Proof.
 apply: (anti_symm _).
 - rewrite public_eq minted_TKey; iDestruct 1 as "[Ht publ]".
-  iDestruct "publ" as "[publ | [(? & _) | [(? & _) | publ]]]" => //.
+  iDestruct "publ" as "[publ | [(? & _) | [(? & _) | [(? & _) | publ]]]]" => //.
   + iDestruct "publ" as (T) "[%dec publ]".
     case: dec => //= {}kt {}t -> [-> ->].
     by rewrite big_sepS_singleton; eauto.
@@ -900,7 +1060,7 @@ Proof.
 apply: (anti_symm _).
 - rewrite public_eq minted_TSeal.
   iDestruct 1 as "[[Hk Ht] publ]".
-  iDestruct "publ" as "[publ | [(? & _) | [(? & _) | publ]]]" => //.
+  iDestruct "publ" as "[publ | [(? & _) | [(? & _) | [(? & _) | publ]]]]" => //.
   + iDestruct "publ" as (T) "[%dec ?]".
     case: dec => // {}k {}t -> [-> ->].
     by rewrite big_sepS_union_pers !big_sepS_singleton; iLeft.
@@ -936,7 +1096,7 @@ Lemma public_THash t :
 Proof.
 apply: (anti_symm _).
 - rewrite public_eq minted_THash.
-  iDestruct 1 as "[Ht [publ | [(? & _) | [(? & _) | publ]]]]" => //; eauto.
+  iDestruct 1 as "[Ht [publ | [(? & _) | [(? & _) | [(? & _) | publ]]]]]" => //; eauto.
   iDestruct "publ" as (T) "[%dec ?]".
   case: dec => //= {}t -> [->].
   by rewrite big_sepS_singleton; eauto.
@@ -965,7 +1125,7 @@ Proof.
 Qed.
 
 Lemma public_TExpN t ts :
-  negb (is_exp t) → negb (is_mul t) → negb (is_inv t) →
+  negb (is_exp t) → negb (is_gmul t) → negb (is_ginv t) →
   invs_canceled ts ->
   ts ≠ [] →
   public (TExpN t ts) ⊣⊢
@@ -983,7 +1143,7 @@ apply: anti_symm; last first.
 - iIntros "#[m dhp]".
   rewrite public_eq; setoid_rewrite (exps_TExpN Nx Nm Ni ic).
   iSplit; first done.
-  iRight; iRight; iLeft.
+  iRight; iRight; iRight; iLeft.
   iSplit; first done.
   iApply (big_sepL_mono with "dhp").
   iIntros (k t' Hk) "H"; iSplit; last by [].
@@ -993,13 +1153,17 @@ apply: anti_symm; last first.
   setoid_rewrite (exps_TExpN Nx Nm Ni ic).
   iIntros "#[[mt mts] Hdisj]".
   iSplit; first by iSplit.
-  iDestruct "Hdisj" as "[c1 | [c2 | [c3 | c4]]]".
+  iDestruct "Hdisj" as "[c1 | [c2 | [c2' | [c3 | c4]]]]".
   + iDestruct "c1" as (T) "[%dec _]".
     by move: ttsX; rewrite (decompose_is_exp dec).
   + iDestruct "c2" as "(%mul_c & _)".
     by move: ttsX mul_c;
        rewrite is_exp_unfold is_mul_unfold;
-       case: (unfold_term (TExpN t ts)) => [|||[] ?].
+       case: (unfold_term (TExpN t ts)) => [|||[|] ?].
+  + iDestruct "c2'" as "(%mul_c & _)".
+    by move: ttsX mul_c;
+       rewrite is_exp_unfold is_gmul_unfold;
+       case: (unfold_term (TExpN t ts)) => [|||[|] ?].
   + iDestruct "c3" as "(_ & exp)".
     iApply (big_sepL_mono with "exp"). by iIntros (k t' _) "(_ & $)".
   + iRevert "c4"; case: (TExpN t ts) ttsX => // *; by iIntros "[]".
@@ -1016,7 +1180,7 @@ move => expt; apply: anti_symm; last first.
 - iIntros "#[m dhp]".
   rewrite public_eq.
   iSplit; first done.
-  iRight; iRight; iLeft.
+  iRight; iRight; iRight; iLeft.
   iSplit; first done.
   iApply (big_sepL_mono with "dhp").
   iIntros (k t' Hk) "H"; iSplit; last by [].
@@ -1026,19 +1190,22 @@ move => expt; apply: anti_symm; last first.
 - rewrite public_eq.
   iIntros "#[m Hdisj]".
   iSplit; first done.
-  iDestruct "Hdisj" as "[c1 | [c2 | [c3 | c4]]]".
+  iDestruct "Hdisj" as "[c1 | [c2 | [c2' | [c3 | c4]]]]".
   + iDestruct "c1" as (T) "[%dec _]".
     by move: expt; rewrite (decompose_is_exp dec).
   + iDestruct "c2" as "(%mul_c & _)".
     by move: expt mul_c;
-       rewrite is_exp_unfold is_mul_unfold; case: (unfold_term t) => [|||[] ?].
+       rewrite is_exp_unfold is_mul_unfold; case: (unfold_term t) => [|||[|] ?].
+  + iDestruct "c2'" as "(%mul_c & _)".
+    by move: expt mul_c;
+       rewrite is_exp_unfold is_gmul_unfold; case: (unfold_term t) => [|||[|] ?].
   + iDestruct "c3" as "(_ & exp)".
     iApply (big_sepL_mono with "exp"). by iIntros (k t' _) "(_ & $)".
   + by case: (t) expt => // *; iDestruct "c4" as "[]".
 Qed.
 
 Lemma public_TExp_iff t1 t2 :
-  negb (is_exp t1) → negb (is_mul t1) → negb (is_inv t1) →
+  negb (is_exp t1) → negb (is_gmul t1) → negb (is_ginv t1) →
   negb (is_mul t2) ->
   public (TExp t1 t2) ⊣⊢
   minted t1 ∧ minted t2 ∧ exp_pred t2 (TExp t1 t2) ∧ □ (public t2 → public t1).
@@ -1052,7 +1219,7 @@ by rewrite bi.sep_emp -!bi.and_assoc.
 Qed.
 
 Lemma public_TExp2_iff t1 t2 t3 :
-  negb (is_exp t1) → negb (is_mul t1) → negb (is_inv t1) →
+  negb (is_exp t1) → negb (is_gmul t1) → negb (is_ginv t1) →
   negb (is_mul t2) ->
   negb (is_mul t3) ->
   t2 ≠ TInv t3 ->
@@ -1092,7 +1259,7 @@ by iDestruct "p" as "[_ [dh ?]]" => //; eauto.
 Qed.
 
 Lemma public_TExp_Nmul t1 t2 :
-  negb (is_mul t1) -> negb (is_inv t1) ->
+  negb (is_gmul t1) -> negb (is_ginv t1) ->
   negb (is_mul t2) ->
   public t1 -∗
   public t2 -∗
@@ -1127,12 +1294,12 @@ have comm : TExp (TExp t1 t2) (TInv t) = TExp (TExp t1 (TInv t)) t2.
 rewrite comm; iApply (IH with "p p2").
 - have NmTt : negb (is_mul (TInv t)) by rewrite is_mul_TInv.
   by have [?[??]] := tsize_TExp_TInv NmTt t_t1.
-- by apply: Nmul_TExp.
-- by apply: Ninv_TExp.
+- by apply: Ngmul_TExp.
+- by apply: Nginv_TExp.
 Qed.
 
 Lemma public_TExpN_intro t ts :
-  negb (is_mul t) -> negb (is_inv t) ->
+  negb (is_gmul t) -> negb (is_ginv t) ->
   invs_canceled ts ->
   public t -∗ ([∗ list] t' ∈ ts, public t') -∗ public (TExpN t ts).
 Proof.
@@ -1141,42 +1308,43 @@ elim: ts => [|u us IH] ic; iIntros "#p #pus".
 - by rewrite TExpN0.
 - move: ic => /invs_canceled_cons [_ [Nu atom_us]].
   rewrite -TExp_TExpN big_sepL_cons; iDestruct "pus" as "[#pu #pus']".
-  iApply (public_TExp_Nmul (Nmul_TExp _ _ Nm) (Ninv_TExp _ _ Nm Ni) Nu
+  iApply (public_TExp_Nmul (Ngmul_TExp _ _ Nm) (Nginv_TExp _ _ Nm Ni) Nu
             with "[] pu").
   by iApply (IH atom_us with "p pus'").
 Qed.
 
-(* Unconditional in both arguments.  A product base distributes, and every
-   factor of the result comes from a factor of [t1] ([mem_factors_TMulN]); an
-   inverse base is pushed out through [TExp_TInv]. *)
+(* Unconditional in both arguments.  A group product base distributes, and every
+   group factor of the result comes from a group factor of [t1]
+   ([mem_gfactors_TGMulN]); a group inverse base is pushed out through
+   [TExp_TGInv]. *)
 Lemma public_TExp t1 t2 :
   public t1 -∗ public t2 -∗ public (TExp t1 t2).
 Proof.
 move: t1; elim/term_lt_ind => t1 IH; iIntros "#p1 #p2".
-case Em: (is_mul t1).
-  have Xm : is_mul t1 by rewrite Em.
-  have Nmf : Forall (fun u => negb (is_mul u))
-               ((fun u => TExp u t2) <$> factors t1).
+case Em: (is_gmul t1).
+  have Xm : is_gmul t1 by rewrite Em.
+  have Nmf : Forall (fun u => negb (is_gmul u))
+               ((fun u => TExp u t2) <$> gfactors t1).
     apply/Forall_fmap/list.Forall_forall => u u_t1.
-    by rewrite /compose; apply: Nmul_TExp; exact: Nmul_factors u_t1.
-  rewrite [public (TExp t1 t2)]public_factors; iSplit.
+    by rewrite /compose; apply: Ngmul_TExp; exact: Ngmul_gfactors u_t1.
+  rewrite [public (TExp t1 t2)]public_gfactors; iSplit.
     by iApply all_minted_TExp; iSplit; iApply public_minted.
   rewrite big_sepL_forall; iIntros (k x Hx).
-  have x_in : x ∈ factors (TExp t1 t2) := list_elem_of_lookup_2 _ _ _ Hx.
-  move: x_in; rewrite {1}(TExp_factors t1 t2).
-  move=> /(mem_factors_TMulN _ _ Nmf) /list_elem_of_fmap [u [-> u_t1]].
-  iApply (IH u (tsize_factors_lt _ _ Xm u_t1) with "[] p2").
-  rewrite (public_factors t1); iDestruct "p1" as "[_ #fs]".
+  have x_in : x ∈ gfactors (TExp t1 t2) := list_elem_of_lookup_2 _ _ _ Hx.
+  move: x_in; rewrite {1}(TExp_gfactors t1 t2).
+  move=> /(mem_gfactors_TGMulN _ _ Nmf) /list_elem_of_fmap [u [-> u_t1]].
+  iApply (IH u (tsize_gfactors_lt _ _ Xm u_t1) with "[] p2").
+  rewrite (public_gfactors t1); iDestruct "p1" as "[_ #fs]".
   by iApply (big_sepL_elem_of with "fs").
-have Nm : negb (is_mul t1) by rewrite Em.
-case Ei: (is_inv t1).
-  have Xi : is_inv t1 by rewrite Ei.
-  have -> : TExp t1 t2 = TInv (TExp (TInv t1) t2).
-    by rewrite -TExp_TInv TInvK.
-  rewrite public_TInv.
-  iApply (IH (TInv t1) (tsize_TInv_lt _ Xi) with "[] p2").
-  by rewrite public_TInv.
-have Ni : negb (is_inv t1) by rewrite Ei.
+have Nm : negb (is_gmul t1) by rewrite Em.
+case Ei: (is_ginv t1).
+  have Xi : is_ginv t1 by rewrite Ei.
+  have -> : TExp t1 t2 = TGInv (TExp (TGInv t1) t2).
+    by rewrite -TExp_TGInv TGInvK.
+  rewrite public_TGInv.
+  iApply (IH (TGInv t1) (tsize_TGInv_lt _ Xi) with "[] p2").
+  by rewrite public_TGInv.
+have Ni : negb (is_ginv t1) by rewrite Ei.
 rewrite (_ : TExp t1 t2 = TExpN t1 (factors t2)); last by rewrite /TExpN factorsK.
 iApply (public_TExpN_intro Nm Ni (invs_canceled_factors t2) with "p1").
 case E: (is_mul t2).
@@ -1185,23 +1353,25 @@ case E: (is_mul t2).
   by rewrite (factors_Nmul _ Hmul) /= bi.sep_emp; iApply "p2".
 Qed.
 
-(* Distributivity, as a publicity principle: [TExp t1 t2] is the product of the
-   [TExp u t2] for [u] a factor of [t1], so it is public exactly when each of
-   those is.  For an atom-headed [t1] this degenerates to the single factor
-   [t1] itself ([factors t1 = [t1]]), so it subsumes the atomic reasoning. *)
-Lemma public_TExp_factors t1 t2 :
-  ([∗ list] u ∈ factors t1, public (TExp u t2)) -∗
+(* Distributivity, as a publicity principle: [TExp t1 t2] is the group product
+   of the [TExp u t2] for [u] a group factor of [t1], so it is public exactly
+   when each of those is.  For a group-atom-headed [t1] this degenerates to the
+   single factor [t1] itself ([gfactors t1 = [t1]]), so it subsumes the atomic
+   reasoning. *)
+Lemma public_TExp_gfactors t1 t2 :
+  ([∗ list] u ∈ gfactors t1, public (TExp u t2)) -∗
   public (TExp t1 t2).
 Proof.
 iIntros "#H".
-have Nmf : Forall (fun v => negb (is_mul v)) ((fun u => TExp u t2) <$> factors t1).
+have Nmf : Forall (fun v => negb (is_gmul v))
+             ((fun u => TExp u t2) <$> gfactors t1).
   apply/Forall_fmap/list.Forall_forall => u u_t1.
-  by rewrite /compose; apply: Nmul_TExp; exact: Nmul_factors u_t1.
-have factE : forall x, x ∈ factors (TExp t1 t2) ->
-    exists u, x = TExp u t2 /\ u ∈ factors t1.
-  move=> x; rewrite {1}(TExp_factors t1 t2).
-  by move=> /(mem_factors_TMulN _ _ Nmf) /list_elem_of_fmap [u [-> u_t1]]; eauto.
-rewrite [public (TExp t1 t2)]public_factors [minted (TExp t1 t2)]minted_factors.
+  by rewrite /compose; apply: Ngmul_TExp; exact: Ngmul_gfactors u_t1.
+have factE : forall x, x ∈ gfactors (TExp t1 t2) ->
+    exists u, x = TExp u t2 /\ u ∈ gfactors t1.
+  move=> x; rewrite {1}(TExp_gfactors t1 t2).
+  by move=> /(mem_gfactors_TGMulN _ _ Nmf) /list_elem_of_fmap [u [-> u_t1]]; eauto.
+rewrite [public (TExp t1 t2)]public_gfactors [minted (TExp t1 t2)]minted_gfactors.
 iSplit; iApply big_sepL_forall; iIntros (k x Hx);
   case: (factE x (list_elem_of_lookup_2 _ _ _ Hx)) => u [-> u_t1].
 - by iApply public_minted; iApply (big_sepL_elem_of with "H").
@@ -1253,6 +1423,53 @@ Proof.
 by iApply (public_TMulN_intro invs_canceled0).
 Qed.
 
+Lemma public_TGMulN_intro ts :
+  ginvs_canceled ts ->
+  ([∗ list] t' ∈ ts, public t') ⊢ public (TGMulN ts).
+Proof.
+move => ic.
+rewrite public_gfactors (gfactors_TGMulN _ ic) minted_TGMulN //.
+iIntros "#H"; iSplit; last done.
+iApply (big_sepL_mono with "H"); iIntros (k t' _) "?"; by iApply public_minted.
+Qed.
+
+Lemma mem_gfactors_TGMulN2 t1 t2 t' :
+  t' ∈ gfactors (TGMulN (t1 :: t2 :: nil)) → t' ∈ gfactors t1 ++ gfactors t2.
+Proof.
+by rewrite elem_of_app -!gcount_gt0 gcount_TGMulN /fmap /=; lia.
+Qed.
+
+Lemma big_sepL_gfactors_TGMulN2
+  (Φ : term → iProp) `{!∀ t, Persistent (Φ t)} t1 t2 :
+  ([∗ list] t' ∈ gfactors t1, Φ t') -∗
+  ([∗ list] t' ∈ gfactors t2, Φ t') -∗
+  [∗ list] t' ∈ gfactors (TGMulN (t1 :: t2 :: nil)), Φ t'.
+Proof.
+iIntros "#H1 #H2"; iApply big_sepL_intro; iIntros "!>" (k u Hk).
+move: (mem_gfactors_TGMulN2 (list_elem_of_lookup_2 _ _ _ Hk))
+  => /elem_of_app[Hin|Hin].
+- by iApply (big_sepL_elem_of with "H1").
+- by iApply (big_sepL_elem_of with "H2").
+Qed.
+
+Lemma public_TGMulN2 t1 t2 :
+  public t1 -∗ public t2 -∗ public (TGMulN (t1 :: t2 :: nil)).
+Proof.
+iIntros "#p1 #p2".
+iDestruct (public_gfactors t1 with "p1") as "#[m1 f1]".
+iDestruct (public_gfactors t2 with "p2") as "#[m2 f2]".
+iEval (rewrite minted_gfactors) in "m1".
+iEval (rewrite minted_gfactors) in "m2".
+iApply public_gfactors; iSplit.
+- rewrite minted_gfactors. by iApply (big_sepL_gfactors_TGMulN2 with "m1 m2").
+- by iApply (big_sepL_gfactors_TGMulN2 with "f1 f2").
+Qed.
+
+Lemma public_TGMul0 : ⊢ public (TGMulN nil).
+Proof.
+by iApply (public_TGMulN_intro ginvs_canceled0).
+Qed.
+
 Lemma False_public t :
   minted t -∗
   ▷ False -∗
@@ -1284,8 +1501,8 @@ case: t IH => [n|ta tb|a|kt tt|kk tt|tt|pt wf nf] IH.
   rewrite minted_THash public_THash.
   iIntros "#m #contra"; iLeft.
   iApply (IH tt H1 with "m contra").
-- case: pt wf nf IH => [o|[kt'||] operand|[||] b e|[] ts] wf nf IH.
-  1,2,3,5,6: by move: {IH} nf; rewrite /is_non_free /=.
+- case: pt wf nf IH => [o|[kt'|||] operand|[||] b e|[|] ts] wf nf IH.
+  1,2,3,6,7: by move: {IH} nf; rewrite /is_non_free /=.
   + have /andb_True [/andb_True [Ninvpt Nmpt] wfpt] := wf.
     have E : TNonFree (PreTerm.PT1 O1Inv operand) wf nf = TInv (fold_term operand).
       apply: unfold_term_inj.
@@ -1300,13 +1517,30 @@ case: t IH => [n|ta tb|a|kt tt|kk tt|tt|pt wf nf] IH.
     iEval (rewrite minted_TInv) in "m".
     rewrite public_TInv.
     iApply (IH (fold_term operand) Hlt with "m contra").
+  + have /andb_True [/andb_True [Ninvpt Nmpt] wfpt] := wf.
+    have E : TNonFree (PreTerm.PT1 O1GInv operand) wf nf
+           = TGInv (fold_term operand).
+      apply: unfold_term_inj.
+      by rewrite unfold_TGInv (fold_termK operand wfpt)
+         (PreTerm.ginv_Ngmul operand Nmpt) (PreTerm.ginv_invN operand Ninvpt).
+    have Ninv : negb (is_ginv (fold_term operand))
+      by rewrite is_ginv_unfold (fold_termK operand wfpt).
+    have Nmf : negb (is_gmul (fold_term operand))
+      by rewrite is_gmul_unfold (fold_termK operand wfpt).
+    have Hlt : tsize (fold_term operand) < tsize (TGInv (fold_term operand)).
+      rewrite (tsize_TGInv _ Nmf Ninv); lia.
+    rewrite E in IH *.
+    iIntros "#m #contra".
+    iEval (rewrite minted_TGInv) in "m".
+    rewrite public_TGInv.
+    iApply (IH (fold_term operand) Hlt with "m contra").
   + set t := TNonFree (PreTerm.PTExp b e) wf nf.
     have xt : is_exp t by [].
     have Nxb : negb (is_exp (base t)) := base_Nexp t.
-    have Nmb : negb (is_mul (base t)).
-      by rewrite is_mul_base; exact: (is_exp_Nmul _ xt).
-    have Nib : negb (is_inv (base t)).
-      by rewrite is_inv_base; exact: (is_exp_Ninv _ xt).
+    have Nmb : negb (is_gmul (base t)).
+      by rewrite is_gmul_base; exact: (is_exp_Ngmul _ xt).
+    have Nib : negb (is_ginv (base t)).
+      by rewrite is_ginv_base; exact: (is_exp_Nginv _ xt).
     have icx : invs_canceled (exps t) := invs_canceled_factors (expo t).
     iIntros "#mt #contra".
     iEval (rewrite -(base_expsK t) (minted_TExpN Nxb Nmb Nib icx)) in "mt".
@@ -1328,6 +1562,16 @@ case: t IH => [n|ta tb|a|kt tt|kk tt|tt|pt wf nf] IH.
     iApply (big_sepL_impl with "mt").
     iIntros "!>" (k ff ff_lk) "#mff".
     iApply (IH ff (tsize_factors_lt _ _ xt (list_elem_of_lookup_2 _ _ _ ff_lk)) with "mff contra").
+  + set t := TNonFree (PreTerm.PTGMul ts) wf nf.
+    have xt : is_gmul t by [].
+    have wfl : ginvs_canceled (gfactors t) := ginvs_canceled_gfactors t.
+    iIntros "#mt #contra".
+    iEval (rewrite -(gfactorsK t)).
+    iApply (public_TGMulN_intro wfl).
+    iEval (rewrite -(gfactorsK t) (minted_TGMulN wfl)) in "mt".
+    iApply (big_sepL_impl with "mt").
+    iIntros "!>" (k ff ff_lk) "#mff".
+    iApply (IH ff (tsize_gfactors_lt _ _ xt (list_elem_of_lookup_2 _ _ _ ff_lk)) with "mff contra").
 Qed.
 
 Lemma except_0_public t :
@@ -1352,7 +1596,7 @@ have t1_nin : t1 ∉ factors t3 by rewrite factors_Nmul // list_elem_of_singleto
 have := not_elem_of_count _ _ t1_nin.
 move: t1V_t2.
 rewrite /exps -!count_gt0
-  (count_expo_TExp _ _ _ (is_exp_Nmul _ xt2) (is_exp_Ninv _ xt2)).
+  (count_expo_TExp _ _ _ (is_exp_Ngmul _ xt2) (is_exp_Nginv _ xt2)).
 rewrite !count_TInv_l count_TInv.
 lia.
 Qed.
@@ -1368,15 +1612,15 @@ iApply exp_pred_ind.
 - iIntros "!> %ts %t1 %t2 %atom_ts %ts_t2 #pts #dh %t3_t2 #p3".
   have Nm3 : negb (is_mul t3) := proj2 (invs_canceled_factors (expo t2) _ t3_t2).
   have xt2 := is_exp_of_exps t3_t2.
-  have Nm2 := is_exp_Nmul _ xt2; have Ni2 := is_exp_Ninv _ xt2.
+  have Nm2 := is_exp_Ngmul _ xt2; have Ni2 := is_exp_Nginv _ xt2.
   have t3V_nin : TInv t3 ∉ ts.
     move=> t3V_ts; move: (ts_t2 _ t3V_ts); rewrite TInvK => H.
     exact: H t3_t2.
   iApply (@exp_pred_intro1_gen _ _ (t3 :: ts)).
   + by apply/invs_canceled_cons; split; last split.
   + move=> t t_ts; case: (decide (t = t3)) => [->|t_t3].
-      rewrite (not_elem_of_TInv_exps Nm3 (Nmul_TExp _ _ Nm2)
-               (Ninv_TExp _ _ Nm2 Ni2)).
+      rewrite (not_elem_of_TInv_exps Nm3 (Ngmul_TExp _ _ Nm2)
+               (Nginv_TExp _ _ Nm2 Ni2)).
       by rewrite TExpKV.
     have {}t_ts: t ∈ ts by case/elem_of_cons: t_ts => //; congruence.
     have t_t2 := ts_t2 _ t_ts.
@@ -1402,8 +1646,8 @@ iApply exp_pred_ind.
     by rewrite !TExp_TExpN TExpNC2.
   rewrite comm; iApply exp_pred_intro2.
   + exact: Nmt.
-  + exact: (Nmul_TExp _ _ Nm_t2).
-  + exact: (Ninv_TExp _ _ Nm_t2 Ni_t2).
+  + exact: (Ngmul_TExp _ _ Nm_t2).
+  + exact: (Nginv_TExp _ _ Nm_t2 Ni_t2).
   + exact: (exp_pred_intro4_aux (not_eq_sym t_t3) t3_t2 t_t2).
   + by iApply "IH1" => //.
   + by iApply "IH2" => //.
@@ -1411,7 +1655,7 @@ iApply exp_pred_ind.
 Qed.
 
 Lemma public_TExp_add t1 t2 :
-  negb (is_mul t1) → negb (is_inv t1) →
+  negb (is_gmul t1) → negb (is_ginv t1) →
   negb (is_mul t2) →
   TInv t2 ∉ exps t1 →
   public t1 -∗
@@ -1445,8 +1689,8 @@ have Nmt : negb (is_mul t) := proj2 (invs_canceled_factors (expo t1) _ t_t1).
 have NmIt : negb (is_mul (TInv t)) by rewrite is_mul_TInv.
 rewrite TExpC; iApply (IH with "p1' m []").
 - by have [_ [_ ?]] := tsize_TExp_TInv NmIt t_t1.
-- exact: (Nmul_TExp _ _ Nm1).
-- exact: (Ninv_TExp _ _ Nm1 Ni1).
+- exact: (Ngmul_TExp _ _ Nm1).
+- exact: (Nginv_TExp _ _ Nm1 Ni1).
 - exact: Nm2.
 - exact: Nm2'.
 - have t2_tV : t2 ≠ TInv t by move=> contra; apply: t2_t1; rewrite contra TInvK.
@@ -1458,7 +1702,7 @@ rewrite TExpC; iApply (IH with "p1' m []").
 Qed.
 
 Lemma public_TExp_exp_pred t1 t2 :
-  negb (is_mul t1) → negb (is_inv t1) →
+  negb (is_gmul t1) → negb (is_ginv t1) →
   negb (is_mul t2) →
   public t1 -∗
   minted t2 -∗
